proof/invariant-abstract/CSpaceInvPre_AI.thy
@@ -1,0 +1,128 @@
+(*
+ * Copyright 2014, General Dynamics C4 Systems
+ *
+ * This software may be distributed and modified according to the terms of
+ * the GNU General Public License version 2. Note that NO WARRANTY is provided.
+ * See "LICENSE_GPLv2.txt" for details.
+ *
+ * @TAG(GD_GPL)
+ *)
+
+theory CSpaceInvPre_AI
+imports "./$L4V_ARCH/ArchAcc_AI"
+begin
+
+unqualify_consts (in Arch)
+  table_cap_ref :: "cap \<Rightarrow> vs_ref list option"
+
+lemma set_cap_caps_of_state[wp]:
+  "\<lbrace>\<lambda>s. P ((caps_of_state s) (ptr \<mapsto> cap))\<rbrace> set_cap cap ptr \<lbrace>\<lambda>rv s. P (caps_of_state s)\<rbrace>"
+  apply (cases ptr)
+  apply (clarsimp simp add: set_cap_def split_def)
+  apply (rule hoare_seq_ext [OF _ get_object_sp])
+  apply (case_tac obj, simp_all add: set_object_def
+                          split del: split_if cong: if_cong bind_cong)
+   apply (rule hoare_pre, wp)
+   apply (clarsimp elim!: rsubst[where P=P]
+                    simp: caps_of_state_cte_wp_at cte_wp_at_cases
+                          fun_upd_def[symmetric] wf_cs_upd obj_at_def
+                  intro!: ext)
+   apply auto[1]
+  apply (rule hoare_pre, wp)
+  apply (clarsimp simp: obj_at_def)
+  apply (safe elim!: rsubst[where P=P] intro!: ext)
+      apply (auto simp: caps_of_state_cte_wp_at cte_wp_at_cases,
+             auto simp: tcb_cap_cases_def split: split_if_asm)
+  done
+
+lemmas obj_irq_refs_Int_not =
+    arg_cong [where f=Not, OF obj_irq_refs_Int, simplified, symmetric]
+
+lemma obj_irq_refs_inD:
+  "x \<in> obj_irq_refs cap \<Longrightarrow> obj_irq_refs cap = {x}"
+  apply (case_tac cap, simp_all add: obj_irq_refs_def cap_irqs_def
+                                     cap_irq_opt_def split: sum.split_asm)
+  apply clarsimp
+  done
+
+lemma objirqrefs_distinct_or_equal:
+  "\<lbrakk> obj_irq_refs cap \<inter> obj_irq_refs cap' \<noteq> {} \<rbrakk> 
+     \<Longrightarrow> obj_irq_refs cap = obj_irq_refs cap'"
+  by (clarsimp elim!: nonemptyE dest!: obj_irq_refs_inD)
+
+lemma obj_ref_is_obj_irq_ref:
+  "x \<in> obj_refs cap \<Longrightarrow> Inl x \<in> obj_irq_refs cap"
+  by (simp add: obj_irq_refs_def)
+
+lemma obj_irq_refs_eq:
+  "(obj_irq_refs cap = obj_irq_refs cap')
+      = (obj_refs cap = obj_refs cap' \<and> cap_irqs cap = cap_irqs cap')"
+  apply (simp add: obj_irq_refs_def)
+  apply (subgoal_tac "\<forall>x y. Inl x \<noteq> Inr y")
+   apply blast
+  apply simp
+  done
+
+lemma not_final_another':
+  "\<lbrakk> \<not> is_final_cap' cap s; fst (get_cap p s) = {(cap, s)};
+       obj_irq_refs cap \<noteq> {} \<rbrakk>
+      \<Longrightarrow> \<exists>p' cap'. p' \<noteq> p \<and> fst (get_cap p' s) = {(cap', s)}
+                         \<and> obj_irq_refs cap' = obj_irq_refs cap
+                         \<and> \<not> is_final_cap' cap' s"
+  apply (simp add: is_final_cap'_def obj_irq_refs_Int_not cong: conj_cong
+              del: split_paired_Ex split_paired_All)
+  apply (erule not_singleton_oneE[where p=p])
+   apply simp
+  apply (rule_tac x=p' in exI)
+  apply clarsimp
+  apply (drule objirqrefs_distinct_or_equal)
+  apply simp
+  done
+
+lemma not_final_another_caps:
+  "\<lbrakk> \<not> is_final_cap' cap s; caps_of_state s p = Some cap;
+       r \<in> obj_irq_refs cap \<rbrakk>
+      \<Longrightarrow> \<exists>p' cap'. p' \<noteq> p \<and> caps_of_state s p' = Some cap'
+                         \<and> obj_irq_refs cap' = obj_irq_refs cap
+                         \<and> \<not> is_final_cap' cap' s"
+  apply (clarsimp dest!: caps_of_state_cteD
+                   simp: cte_wp_at_def)
+  apply (drule(1) not_final_another')
+   apply clarsimp
+  apply clarsimp
+  apply (subgoal_tac "cte_wp_at (op = cap') (a, b) s")
+   apply (fastforce simp: cte_wp_at_caps_of_state)
+  apply (simp add: cte_wp_at_def)
+  done
+
+lemma wf_cs_ran_nonempty:
+  "well_formed_cnode_n sz cs \<Longrightarrow> ran cs \<noteq> {}"
+  apply (clarsimp simp: well_formed_cnode_n_def)
+  apply (drule_tac f="\<lambda>S. replicate sz False \<in> S" in arg_cong)
+  apply (auto intro: ranI)
+  done
+
+lemma set_cap_obj_at_impossible:
+  "\<lbrace>\<lambda>s. P (obj_at P' p s) \<and> (\<forall>ko. P' ko \<longrightarrow> caps_of ko = {})\<rbrace>
+     set_cap cap ptr
+   \<lbrace>\<lambda>rv s. P (obj_at P' p s)\<rbrace>"
+  apply (simp add: set_cap_def split_def set_object_def)
+  apply (wp get_object_wp | wpc)+
+  apply (clarsimp simp: obj_at_def)
+  apply (subgoal_tac "\<forall>sz cs. well_formed_cnode_n sz cs \<longrightarrow> \<not> P' (CNode sz cs)")
+   apply (subgoal_tac "\<forall>tcb. \<not> P' (TCB tcb)")
+    apply (clarsimp simp: fun_upd_def[symmetric] wf_cs_insert dom_def)
+    apply auto[1]
+   apply (auto simp:caps_of_def cap_of_def ran_tcb_cnode_map wf_cs_ran_nonempty)
+  done
+
+definition
+  no_cap_to_obj_with_diff_ref :: "cap \<Rightarrow> cslot_ptr set \<Rightarrow> 'z::state_ext state \<Rightarrow> bool"
+where
+ "no_cap_to_obj_with_diff_ref cap S \<equiv>
+  \<lambda>s. \<forall>p \<in> UNIV - S. \<not> cte_wp_at (\<lambda>c. obj_refs c = obj_refs cap \<and>
+                                     \<not> (table_cap_ref c = table_cap_ref cap)) p s"
+                                                 
+
+
+end
