proof/invariant-abstract/CSpace_AI.thy
@@ -3639,7 +3639,7 @@ lemma set_free_index_invs:
   apply wps
   
   apply (wp hoare_vcg_all_lift set_cap_irq_handlers set_cap_arch_objs set_cap_valid_arch_caps
-    set_cap_valid_global_objs set_cap_irq_handlers cap_table_at_lift_valid set_cap_typ_at )
+    set_cap.valid_global_objs set_cap_irq_handlers cap_table_at_lift_valid set_cap_typ_at )
   apply (clarsimp simp:cte_wp_at_caps_of_state)
   apply (rule conjI,simp add:valid_pspace_def)
   apply (rule conjI,clarsimp simp:is_cap_simps)
